\begin{itemize}
\item[Case:] commuting conversion cut vs cut (first case).
  The following proof
  \begin{center}
    \begin{math}
      $$\mprset{flushleft}
      \inferrule* [right=Cut] {
        $$\mprset{flushleft}
        \inferrule* [right=] {
          \inferrule* [right=,vdots=1.5em,fraction=\,] {
            \,
          }{\pi_1}
        }{[[G1 |- t : A]]}
        \\
        $$\mprset{flushleft}
        \inferrule* [right=Cut] {
          $$\mprset{flushleft}
          \inferrule* [right=] {
            \inferrule* [right=,vdots=1.5em,fraction=\,] {
              \,
            }{\pi_2}
          }{[[x : A,G2 |- t1 : B]]}
          \\
          $$\mprset{flushleft}
          \inferrule* [right=] {
            \inferrule* [right=,vdots=1.5em,fraction=\,] {
              \,
            }{\pi_3}
          }{[[y : B,G3 |- t' : C]]}
        }{[[x : A,G2,G3 |- [t1/y]t' : C]]}
      }{[[G1,G2,G3 |- [t/x][t1/y]t' : C]]}
    \end{math}
  \end{center}
  is transformed into the proof
  \begin{center}
    \begin{math}
      $$\mprset{flushleft}
      \inferrule* [right=Cut] {
        $$\mprset{flushleft}
        \inferrule* [right=] {
          $$\mprset{flushleft}
          \inferrule* [right=] {
            \inferrule* [right=,vdots=1.5em,fraction=\,] {
              \,
            }{\pi_1}               
          }{[[G1 |- t : A]]}
          \\
          $$\mprset{flushleft}
          \inferrule* [right=] {
            \inferrule* [right=,vdots=1.5em,fraction=\,] {
              \,
            }{\pi_2}
          }{[[x : A,G2 |- t1 : B]]}
        }{[[G1,G2 |- [t/x]t1 : B]]}
        \\
        $$\mprset{flushleft}
        \inferrule* [right=] {
          \inferrule* [right=,vdots=1.5em,fraction=\,] {
            \,
          }{\pi_3}
        }{[[y : B,G3 |- t' : C]]}
      }{[[G1,G2,G3 |- [ [t/x]t1/y]t' : C]]}
    \end{math}
  \end{center}

%% ******* Doesn't hold in non-commutative case:
%% 
%% \item[Case:] commuting conversion cut vs. cut (second case).  The second commuting conversion on cut begins with the proof
%%   \begin{center}
%%     \begin{math}
%%       $$\mprset{flushleft}
%%       \inferrule* [right=Cut] {
%%         $$\mprset{flushleft}
%%         \inferrule* [right=] {
%%           \inferrule* [right=,vdots=1.5em,fraction=\,] {
%%             \,
%%           }{\pi_1}
%%         }{[[G |- t : A]]}
%%         \\
%%         $$\mprset{flushleft}
%%         \inferrule* [right=Cut] {
%%           $$\mprset{flushleft}
%%           \inferrule* [right=] {
%%             \inferrule* [right=,vdots=1.5em,fraction=\,] {
%%               \,
%%             }{\pi_2}
%%           }{[[G' |- t' : B]]}
%%           \\
%%           $$\mprset{flushleft}
%%           \inferrule* [right=] {
%%             \inferrule* [right=,vdots=1.5em,fraction=\,] {
%%               \,
%%             }{\pi_3}
%%           }{[[x : A,G2,y:B,G3 |- t'' : C]]}
%%         }{[[G1,x : A,G2,G',G3 |- [t'/y]t'' : C]]}
%%       }{[[G1,G,G2,G',G3 |- [t/x][t'/y]t'' : C]]}
%%     \end{math}
%%   \end{center}
%%   is transformed into the following proof:
%%   \begin{center}
%%     \begin{math}
%%       $$\mprset{flushleft}
%%       \inferrule* [right=Cut] {
%%         $$\mprset{flushleft}
%%         \inferrule* [right=] {
%%           \inferrule* [right=,vdots=1.5em,fraction=\,] {
%%             \,
%%           }{\pi_2}
%%         }{[[G' |- t' : B]]}
%%         \\
%%         $$\mprset{flushleft}
%%         \inferrule* [right=Cut] {
%%           $$\mprset{flushleft}
%%           \inferrule* [right=] {
%%             \inferrule* [right=,vdots=1.5em,fraction=\,] {
%%               \,
%%             }{\pi_1}
%%           }{[[G |- t : A]]}      
%%           \\
%%           $$\mprset{flushleft}
%%           \inferrule* [right=] {
%%             \inferrule* [right=,vdots=1.5em,fraction=\,] {
%%               \,
%%             }{\pi_3}
%%           }{[[G1,x : A,G2,y:B,G3 |- t'' : C]]}
%%         }{[[G1,G,G2,y:B,G3 |- [t/x]t'' : C]]}
%%       }{[[G1,G,G2,G',G3 |- [t'/y][t/x]t'' : C]]}
%%     \end{math}
%%   \end{center}
  

\item[Case:] the $\eta$-expansion cases: tensor.  
  The proof
  \begin{center}
    \begin{math}
      $$\mprset{flushleft}
      \inferrule* [right=Ax] {
        \,
      }{[[x : A (x) B |- x : A (x) B]]}
    \end{math}
  \end{center}
  is transformed into the proof
  \begin{center}
    \begin{math}
      $$\mprset{flushleft}
      \inferrule* [right=Tl] {
        $$\mprset{flushleft}
        \inferrule* [right=Tr] {
          $$\mprset{flushleft}
          \inferrule* [right=Ax] {
            \,
          }{[[y : A |- y : A]]}
          \\
          $$\mprset{flushleft}
          \inferrule* [right=Ax] {
            \,
          }{[[z : B |- z : B]]}
        }{[[y : A, z : B |- y (x) z : A (x) B]]}
      }{[[x : A (x) B |- let x be y (x) z in {y (x) z} : A (x) B]]}
    \end{math}
  \end{center}

\item[Case:] the $\eta$-expansion cases: implication.
  The proof
  \begin{center}
    \begin{math}
      $$\mprset{flushleft}
      \inferrule* [right=T\_Var] {
        \,
      }{[[x : A -> B |- x : A -> B]]}
    \end{math}
  \end{center}
  transforms into the proof 
  \begin{center}
    \begin{math}
      $$\mprset{flushleft}
      \inferrule* [right=T\_IRl] {
        $$\mprset{flushleft}
        \inferrule* [right=T\_IRr] {
          $$\mprset{flushleft}
          \inferrule* [right=T\_Var] {
            \,
          }{[[y : A |- y : A]]}
          \\
          $$\mprset{flushleft}
          \inferrule* [right=T\_Var] {
            \,
          }{[[z : B |- z : B]]}
        }{[[y : A, x : A -> B |- appr x y : B]]}
      }{[[x : A -> B |- \r y:A.appr x y : A -> B]]}
    \end{math}  
  \end{center}

\item[Case:] the $\eta$-expansion cases: implication.
  The proof
  \begin{center}
    \begin{math}
      $$\mprset{flushleft}
      \inferrule* [right=T\_Var] {
        \,
      }{[[x : B <- A |- x : B <- A]]}
    \end{math}
  \end{center}
  transforms into the proof 
  \begin{center}
    \begin{math}
      $$\mprset{flushleft}
      \inferrule* [right=T\_ILl] {
        $$\mprset{flushleft}
        \inferrule* [right=T\_ILr] {
          $$\mprset{flushleft}
          \inferrule* [right=T\_Var] {
            \,
          }{[[y : A |- y : A]]}
          \\
          $$\mprset{flushleft}
          \inferrule* [right=T\_Var] {
            \,
          }{[[z : B |- z : B]]}
        }{[[y : A, x : B <- A |- appl x y : B]]}
      }{[[x : B <- A |- \l y:A.appl x y : A <- B]]}
    \end{math}  
  \end{center}  
  
\item[Case:] the $\eta$-expansion cases: tensor unit.
  The proof
  \begin{center}
    \begin{math}
      $$\mprset{flushleft}
      \inferrule* [right=Var] {
        \,
      }{[[x : I |- x : I]]}
    \end{math}
  \end{center}
  transforms into the proof
  \begin{center}
    \begin{math}
      $$\mprset{flushleft}
      \inferrule* [right=Ul] {
        $$\mprset{flushleft}
        \inferrule* [right=Ur] {
          \,
        }{[[. |- unit : I]]}
      }{[[x : I |- let x be punit in unit : I]]}
    \end{math}
  \end{center}

\item[Case:] the axiom steps: the axiom step. The proof 
  \begin{center}
    \begin{math}
      $$\mprset{flushleft}
      \inferrule* [right=T\_Cut] {
        $$\mprset{flushleft}
        \inferrule* [right=T\_Var] {
          \,
        }{[[x : A |- x : A]]}
        \\
        $$\mprset{flushleft}
        \inferrule* [right=] {
          \inferrule* [right=,vdots=1.5em,fraction=\,] {
            \,
          }{\pi}          
        }{[[y : A, G |- t : C]]}
      }{[[x : A, G |- [x/y]t : C]]}
    \end{math}
  \end{center}
  transforms into the proof
  \begin{center}
    \begin{math}
      $$\mprset{flushleft}
      \inferrule* [right=] {
        \inferrule* [right=,vdots=1.5em,fraction=\,] {
          \,
        }{\pi}          
      }{[[y : A, G |- t : C]]}
    \end{math}
  \end{center}
  
\end{itemize}
