\begin{itemize}
\item[Case:] commuting conversion cut vs cut (first case).
  The following proof
  \begin{center}
    \begin{math}
      $$\mprset{flushleft}
      \inferrule* [right=Cut] {
        $$\mprset{flushleft}
        \inferrule* [right=] {
          \inferrule* [right=,vdots=1.5em,fraction=\,] {
            \,
          }{\pi_1}
        }{ \Gamma_{{\mathrm{1}}}  \vdash  \Lnt{t}  :  \Lnt{A} }
        \\
        $$\mprset{flushleft}
        \inferrule* [right=Cut] {
          $$\mprset{flushleft}
          \inferrule* [right=] {
            \inferrule* [right=,vdots=1.5em,fraction=\,] {
              \,
            }{\pi_2}
          }{ \Lmv{x}  \Lsym{:}  \Lnt{A}  \Lsym{,}  \Gamma_{{\mathrm{2}}}  \vdash  \Lnt{t_{{\mathrm{1}}}}  :  \Lnt{B} }
          \\
          $$\mprset{flushleft}
          \inferrule* [right=] {
            \inferrule* [right=,vdots=1.5em,fraction=\,] {
              \,
            }{\pi_3}
          }{ \Lmv{y}  \Lsym{:}  \Lnt{B}  \Lsym{,}  \Gamma_{{\mathrm{3}}}  \vdash  \Lnt{t'}  :  \Lnt{C} }
        }{ \Lmv{x}  \Lsym{:}  \Lnt{A}  \Lsym{,}  \Gamma_{{\mathrm{2}}}  \Lsym{,}  \Gamma_{{\mathrm{3}}}  \vdash  \Lsym{[}  \Lnt{t_{{\mathrm{1}}}}  \Lsym{/}  \Lmv{y}  \Lsym{]}  \Lnt{t'}  :  \Lnt{C} }
      }{ \Gamma_{{\mathrm{1}}}  \Lsym{,}  \Gamma_{{\mathrm{2}}}  \Lsym{,}  \Gamma_{{\mathrm{3}}}  \vdash  \Lsym{[}  \Lnt{t}  \Lsym{/}  \Lmv{x}  \Lsym{]}  \Lsym{[}  \Lnt{t_{{\mathrm{1}}}}  \Lsym{/}  \Lmv{y}  \Lsym{]}  \Lnt{t'}  :  \Lnt{C} }
    \end{math}
  \end{center}
  is transformed into the proof
  \begin{center}
    \begin{math}
      $$\mprset{flushleft}
      \inferrule* [right=Cut] {
        $$\mprset{flushleft}
        \inferrule* [right=] {
          $$\mprset{flushleft}
          \inferrule* [right=] {
            \inferrule* [right=,vdots=1.5em,fraction=\,] {
              \,
            }{\pi_1}               
          }{ \Gamma_{{\mathrm{1}}}  \vdash  \Lnt{t}  :  \Lnt{A} }
          \\
          $$\mprset{flushleft}
          \inferrule* [right=] {
            \inferrule* [right=,vdots=1.5em,fraction=\,] {
              \,
            }{\pi_2}
          }{ \Lmv{x}  \Lsym{:}  \Lnt{A}  \Lsym{,}  \Gamma_{{\mathrm{2}}}  \vdash  \Lnt{t_{{\mathrm{1}}}}  :  \Lnt{B} }
        }{ \Gamma_{{\mathrm{1}}}  \Lsym{,}  \Gamma_{{\mathrm{2}}}  \vdash  \Lsym{[}  \Lnt{t}  \Lsym{/}  \Lmv{x}  \Lsym{]}  \Lnt{t_{{\mathrm{1}}}}  :  \Lnt{B} }
        \\
        $$\mprset{flushleft}
        \inferrule* [right=] {
          \inferrule* [right=,vdots=1.5em,fraction=\,] {
            \,
          }{\pi_3}
        }{ \Lmv{y}  \Lsym{:}  \Lnt{B}  \Lsym{,}  \Gamma_{{\mathrm{3}}}  \vdash  \Lnt{t'}  :  \Lnt{C} }
      }{ \Gamma_{{\mathrm{1}}}  \Lsym{,}  \Gamma_{{\mathrm{2}}}  \Lsym{,}  \Gamma_{{\mathrm{3}}}  \vdash  \Lsym{[}  \Lsym{[}  \Lnt{t}  \Lsym{/}  \Lmv{x}  \Lsym{]}  \Lnt{t_{{\mathrm{1}}}}  \Lsym{/}  \Lmv{y}  \Lsym{]}  \Lnt{t'}  :  \Lnt{C} }
    \end{math}
  \end{center}

%% ******* Doesn't hold in non-commutative case:
%% 
%% \item[Case:] commuting conversion cut vs. cut (second case).  The second commuting conversion on cut begins with the proof
%%   \begin{center}
%%     \begin{math}
%%       $$\mprset{flushleft}
%%       \inferrule* [right=Cut] {
%%         $$\mprset{flushleft}
%%         \inferrule* [right=] {
%%           \inferrule* [right=,vdots=1.5em,fraction=\,] {
%%             \,
%%           }{\pi_1}
%%         }{ \Gamma  \vdash  \Lnt{t}  :  \Lnt{A} }
%%         \\
%%         $$\mprset{flushleft}
%%         \inferrule* [right=Cut] {
%%           $$\mprset{flushleft}
%%           \inferrule* [right=] {
%%             \inferrule* [right=,vdots=1.5em,fraction=\,] {
%%               \,
%%             }{\pi_2}
%%           }{ \Gamma'  \vdash  \Lnt{t'}  :  \Lnt{B} }
%%           \\
%%           $$\mprset{flushleft}
%%           \inferrule* [right=] {
%%             \inferrule* [right=,vdots=1.5em,fraction=\,] {
%%               \,
%%             }{\pi_3}
%%           }{ \Lmv{x}  \Lsym{:}  \Lnt{A}  \Lsym{,}  \Gamma_{{\mathrm{2}}}  \Lsym{,}  \Lmv{y}  \Lsym{:}  \Lnt{B}  \Lsym{,}  \Gamma_{{\mathrm{3}}}  \vdash  \Lnt{t''}  :  \Lnt{C} }
%%         }{ \Gamma_{{\mathrm{1}}}  \Lsym{,}  \Lmv{x}  \Lsym{:}  \Lnt{A}  \Lsym{,}  \Gamma_{{\mathrm{2}}}  \Lsym{,}  \Gamma'  \Lsym{,}  \Gamma_{{\mathrm{3}}}  \vdash  \Lsym{[}  \Lnt{t'}  \Lsym{/}  \Lmv{y}  \Lsym{]}  \Lnt{t''}  :  \Lnt{C} }
%%       }{ \Gamma_{{\mathrm{1}}}  \Lsym{,}  \Gamma  \Lsym{,}  \Gamma_{{\mathrm{2}}}  \Lsym{,}  \Gamma'  \Lsym{,}  \Gamma_{{\mathrm{3}}}  \vdash  \Lsym{[}  \Lnt{t}  \Lsym{/}  \Lmv{x}  \Lsym{]}  \Lsym{[}  \Lnt{t'}  \Lsym{/}  \Lmv{y}  \Lsym{]}  \Lnt{t''}  :  \Lnt{C} }
%%     \end{math}
%%   \end{center}
%%   is transformed into the following proof:
%%   \begin{center}
%%     \begin{math}
%%       $$\mprset{flushleft}
%%       \inferrule* [right=Cut] {
%%         $$\mprset{flushleft}
%%         \inferrule* [right=] {
%%           \inferrule* [right=,vdots=1.5em,fraction=\,] {
%%             \,
%%           }{\pi_2}
%%         }{ \Gamma'  \vdash  \Lnt{t'}  :  \Lnt{B} }
%%         \\
%%         $$\mprset{flushleft}
%%         \inferrule* [right=Cut] {
%%           $$\mprset{flushleft}
%%           \inferrule* [right=] {
%%             \inferrule* [right=,vdots=1.5em,fraction=\,] {
%%               \,
%%             }{\pi_1}
%%           }{ \Gamma  \vdash  \Lnt{t}  :  \Lnt{A} }      
%%           \\
%%           $$\mprset{flushleft}
%%           \inferrule* [right=] {
%%             \inferrule* [right=,vdots=1.5em,fraction=\,] {
%%               \,
%%             }{\pi_3}
%%           }{ \Gamma_{{\mathrm{1}}}  \Lsym{,}  \Lmv{x}  \Lsym{:}  \Lnt{A}  \Lsym{,}  \Gamma_{{\mathrm{2}}}  \Lsym{,}  \Lmv{y}  \Lsym{:}  \Lnt{B}  \Lsym{,}  \Gamma_{{\mathrm{3}}}  \vdash  \Lnt{t''}  :  \Lnt{C} }
%%         }{ \Gamma_{{\mathrm{1}}}  \Lsym{,}  \Gamma  \Lsym{,}  \Gamma_{{\mathrm{2}}}  \Lsym{,}  \Lmv{y}  \Lsym{:}  \Lnt{B}  \Lsym{,}  \Gamma_{{\mathrm{3}}}  \vdash  \Lsym{[}  \Lnt{t}  \Lsym{/}  \Lmv{x}  \Lsym{]}  \Lnt{t''}  :  \Lnt{C} }
%%       }{ \Gamma_{{\mathrm{1}}}  \Lsym{,}  \Gamma  \Lsym{,}  \Gamma_{{\mathrm{2}}}  \Lsym{,}  \Gamma'  \Lsym{,}  \Gamma_{{\mathrm{3}}}  \vdash  \Lsym{[}  \Lnt{t'}  \Lsym{/}  \Lmv{y}  \Lsym{]}  \Lsym{[}  \Lnt{t}  \Lsym{/}  \Lmv{x}  \Lsym{]}  \Lnt{t''}  :  \Lnt{C} }
%%     \end{math}
%%   \end{center}
  

\item[Case:] the $\eta$-expansion cases: tensor.  
  The proof
  \begin{center}
    \begin{math}
      $$\mprset{flushleft}
      \inferrule* [right=Ax] {
        \,
      }{ \Lmv{x}  \Lsym{:}   \Lnt{A}  \otimes  \Lnt{B}   \vdash  \Lmv{x}  :   \Lnt{A}  \otimes  \Lnt{B}  }
    \end{math}
  \end{center}
  is transformed into the proof
  \begin{center}
    \begin{math}
      $$\mprset{flushleft}
      \inferrule* [right=Tl] {
        $$\mprset{flushleft}
        \inferrule* [right=Tr] {
          $$\mprset{flushleft}
          \inferrule* [right=Ax] {
            \,
          }{ \Lmv{y}  \Lsym{:}  \Lnt{A}  \vdash  \Lmv{y}  :  \Lnt{A} }
          \\
          $$\mprset{flushleft}
          \inferrule* [right=Ax] {
            \,
          }{ \Lmv{z}  \Lsym{:}  \Lnt{B}  \vdash  \Lmv{z}  :  \Lnt{B} }
        }{ \Lmv{y}  \Lsym{:}  \Lnt{A}  \Lsym{,}  \Lmv{z}  \Lsym{:}  \Lnt{B}  \vdash   \Lmv{y}  \otimes  \Lmv{z}   :   \Lnt{A}  \otimes  \Lnt{B}  }
      }{ \Lmv{x}  \Lsym{:}   \Lnt{A}  \otimes  \Lnt{B}   \vdash   \mathsf{let}\, \Lmv{x} \,\mathsf{be}\,  \Lmv{y}  \otimes  \Lmv{z}  \,\mathsf{in}\,  (   \Lmv{y}  \otimes  \Lmv{z}   )    :   \Lnt{A}  \otimes  \Lnt{B}  }
    \end{math}
  \end{center}

\item[Case:] the $\eta$-expansion cases: implication.
  The proof
  \begin{center}
    \begin{math}
      $$\mprset{flushleft}
      \inferrule* [right=T\_Var] {
        \,
      }{ \Lmv{x}  \Lsym{:}   \Lnt{A}  \rightharpoonup  \Lnt{B}   \vdash  \Lmv{x}  :   \Lnt{A}  \rightharpoonup  \Lnt{B}  }
    \end{math}
  \end{center}
  transforms into the proof 
  \begin{center}
    \begin{math}
      $$\mprset{flushleft}
      \inferrule* [right=T\_IRl] {
        $$\mprset{flushleft}
        \inferrule* [right=T\_IRr] {
          $$\mprset{flushleft}
          \inferrule* [right=T\_Var] {
            \,
          }{ \Lmv{y}  \Lsym{:}  \Lnt{A}  \vdash  \Lmv{y}  :  \Lnt{A} }
          \\
          $$\mprset{flushleft}
          \inferrule* [right=T\_Var] {
            \,
          }{ \Lmv{z}  \Lsym{:}  \Lnt{B}  \vdash  \Lmv{z}  :  \Lnt{B} }
        }{ \Lmv{y}  \Lsym{:}  \Lnt{A}  \Lsym{,}  \Lmv{x}  \Lsym{:}   \Lnt{A}  \rightharpoonup  \Lnt{B}   \vdash   \mathsf{app}_r\, \Lmv{x} \, \Lmv{y}   :  \Lnt{B} }
      }{ \Lmv{x}  \Lsym{:}   \Lnt{A}  \rightharpoonup  \Lnt{B}   \vdash   \lambda_r  \Lmv{y} : \Lnt{A} .  \mathsf{app}_r\, \Lmv{x} \, \Lmv{y}    :   \Lnt{A}  \rightharpoonup  \Lnt{B}  }
    \end{math}  
  \end{center}

\item[Case:] the $\eta$-expansion cases: implication.
  The proof
  \begin{center}
    \begin{math}
      $$\mprset{flushleft}
      \inferrule* [right=T\_Var] {
        \,
      }{ \Lmv{x}  \Lsym{:}   \Lnt{B}  \leftharpoonup  \Lnt{A}   \vdash  \Lmv{x}  :   \Lnt{B}  \leftharpoonup  \Lnt{A}  }
    \end{math}
  \end{center}
  transforms into the proof 
  \begin{center}
    \begin{math}
      $$\mprset{flushleft}
      \inferrule* [right=T\_ILl] {
        $$\mprset{flushleft}
        \inferrule* [right=T\_ILr] {
          $$\mprset{flushleft}
          \inferrule* [right=T\_Var] {
            \,
          }{ \Lmv{y}  \Lsym{:}  \Lnt{A}  \vdash  \Lmv{y}  :  \Lnt{A} }
          \\
          $$\mprset{flushleft}
          \inferrule* [right=T\_Var] {
            \,
          }{ \Lmv{z}  \Lsym{:}  \Lnt{B}  \vdash  \Lmv{z}  :  \Lnt{B} }
        }{ \Lmv{y}  \Lsym{:}  \Lnt{A}  \Lsym{,}  \Lmv{x}  \Lsym{:}   \Lnt{B}  \leftharpoonup  \Lnt{A}   \vdash   \mathsf{app}_l\, \Lmv{x} \, \Lmv{y}   :  \Lnt{B} }
      }{ \Lmv{x}  \Lsym{:}   \Lnt{B}  \leftharpoonup  \Lnt{A}   \vdash   \lambda_l  \Lmv{y} : \Lnt{A} .  \mathsf{app}_l\, \Lmv{x} \, \Lmv{y}    :   \Lnt{A}  \leftharpoonup  \Lnt{B}  }
    \end{math}  
  \end{center}  
  
\item[Case:] the $\eta$-expansion cases: tensor unit.
  The proof
  \begin{center}
    \begin{math}
      $$\mprset{flushleft}
      \inferrule* [right=Var] {
        \,
      }{ \Lmv{x}  \Lsym{:}   I   \vdash  \Lmv{x}  :   I  }
    \end{math}
  \end{center}
  transforms into the proof
  \begin{center}
    \begin{math}
      $$\mprset{flushleft}
      \inferrule* [right=Ul] {
        $$\mprset{flushleft}
        \inferrule* [right=Ur] {
          \,
        }{  \cdot   \vdash   \mathsf{unit}   :   I  }
      }{ \Lmv{x}  \Lsym{:}   I   \vdash   \mathsf{let}\, \Lmv{x} \,\mathsf{be}\,  \mathsf{unit}  \,\mathsf{in}\,  \mathsf{unit}    :   I  }
    \end{math}
  \end{center}

\item[Case:] the axiom steps: the axiom step. The proof 
  \begin{center}
    \begin{math}
      $$\mprset{flushleft}
      \inferrule* [right=T\_Cut] {
        $$\mprset{flushleft}
        \inferrule* [right=T\_Var] {
          \,
        }{ \Lmv{x}  \Lsym{:}  \Lnt{A}  \vdash  \Lmv{x}  :  \Lnt{A} }
        \\
        $$\mprset{flushleft}
        \inferrule* [right=] {
          \inferrule* [right=,vdots=1.5em,fraction=\,] {
            \,
          }{\pi}          
        }{ \Lmv{y}  \Lsym{:}  \Lnt{A}  \Lsym{,}  \Gamma  \vdash  \Lnt{t}  :  \Lnt{C} }
      }{ \Lmv{x}  \Lsym{:}  \Lnt{A}  \Lsym{,}  \Gamma  \vdash  \Lsym{[}  \Lmv{x}  \Lsym{/}  \Lmv{y}  \Lsym{]}  \Lnt{t}  :  \Lnt{C} }
    \end{math}
  \end{center}
  transforms into the proof
  \begin{center}
    \begin{math}
      $$\mprset{flushleft}
      \inferrule* [right=] {
        \inferrule* [right=,vdots=1.5em,fraction=\,] {
          \,
        }{\pi}          
      }{ \Lmv{y}  \Lsym{:}  \Lnt{A}  \Lsym{,}  \Gamma  \vdash  \Lnt{t}  :  \Lnt{C} }
    \end{math}
  \end{center}
  
\end{itemize}
